Merged a lot, up to instantiation

vipersemabstract/AbstractSemantics.thy
@@ -1,11 +1,178 @@
 theory AbstractSemantics
-  imports ViperCommon.LiftSepAlgebra ViperCommon.SepLogic
+  imports ViperCommon.SepLogic ViperCommon.SepAlgebra ViperCommon.PartialMap ViperCommon.ViperLang
 begin
+
+section \<open>Add a store to the state\<close>
+
+type_synonym 'v ag_store = "(var \<rightharpoonup> 'v) agreement"
+type_synonym ('v, 'a) abs_state = "'v ag_store \<times> 'a"
+
+subsection \<open>Normal states\<close>
+
+(* TODO: rename get_ into abs_? *)
+(* TODO: Should state be renamed to heap? get_abs_state on abs_state sounds like the identity *)
+(* TODO: define this via record instead of getter and setter functions? This would require proving the
+class instances for the record (via isomorphism?), but one would get nice getters and setters automatically *)
+
+definition get_store :: "('v, 'a) abs_state \<Rightarrow> (var \<rightharpoonup> 'v)" where "get_store \<omega> = the_ag (fst \<omega>)"
+definition get_abs_state :: "('v, 'a) abs_state \<Rightarrow> 'a" where "get_abs_state \<omega> = snd \<omega>"
+definition set_store :: "('v, 'a) abs_state \<Rightarrow> (var \<rightharpoonup> 'v) \<Rightarrow> ('v, 'a) abs_state" where
+  "set_store \<omega> s = (Ag s, get_abs_state \<omega>)"
+definition set_abs_state :: "('v, 'a) abs_state \<Rightarrow> 'a \<Rightarrow> ('v, 'a) abs_state" where
+  "set_abs_state \<omega> s = (Ag (get_store \<omega>), s)"
+
+lemma get_store_set_store [simp] :
+  "get_store (set_store \<omega> st) = st"
+  by (simp add:get_store_def set_store_def)
+lemma get_store_set_abs_state [simp] :
+  "get_store (set_abs_state \<omega> st) = get_store \<omega>"
+  by (simp add:get_store_def set_abs_state_def)
+
+lemma get_abs_state_set_store [simp] :
+  "get_abs_state (set_store \<omega> st) = get_abs_state \<omega>"
+  by (simp add:get_abs_state_def set_store_def)
+lemma get_abs_state_set_abs_state [simp] :
+  "get_abs_state (set_abs_state \<omega> st) = st"
+  by (simp add:get_abs_state_def set_abs_state_def)
+
+lemma get_store_stabilize[simp]:
+  "get_store (stabilize \<omega>) = get_store \<omega>"
+  by (metis agreement.collapse fst_conv get_store_def stabilize_ag stabilize_prod_def)
+lemma set_store_stabilize[simp]:
+  "set_store (stabilize \<omega>) s = stabilize (set_store \<omega> s)"
+  by (simp add: get_abs_state_def set_store_def stabilize_ag stabilize_prod_def)
+
+lemma ag_the_ag_same:
+  "a = b \<longleftrightarrow> the_ag a = the_ag b"
+  using agreement.expand by blast
+
+lemma ag_comp:
+  fixes x :: "'v agreement"
+  shows "x ## y \<longleftrightarrow> x = y"
+  by (simp add: defined_def plus_agreement_def)
+
+lemma comp_prod:
+  "a ## b \<longleftrightarrow> (fst a ## fst b \<and> snd a ## snd b)" (is "?A \<longleftrightarrow> ?B")
+proof
+  assume ?A
+  then obtain x where "Some x = a \<oplus> b"
+    by (metis defined_def not_Some_eq)
+  then have "Some (fst x) = fst a \<oplus> fst b \<and> Some (snd x) = snd a \<oplus> snd b"
+    by (metis plus_prodE)
+  then show ?B
+    by (metis defined_def option.discI)
+next
+  assume ?B
+  then obtain r1 r2 where "Some r1 = fst a \<oplus> fst b \<and> Some r2 = snd a \<oplus> snd b"
+    by (metis defined_def option.exhaust_sel)
+  then show ?A
+    using defined_def plus_prodIAlt by fastforce
+qed    
+
+lemma get_store_trace_comp:
+  "fst a ## fst b \<longleftrightarrow> get_store a = get_store b" (is "?A \<longleftrightarrow> ?B")
+  by (simp add: ag_comp ag_the_ag_same comp_prod get_store_def)
+
+lemma plus_state_def:
+  "\<omega>1 \<oplus> \<omega>2 = (let r = (get_abs_state \<omega>1 \<oplus> get_abs_state \<omega>2) in
+  (if get_store \<omega>1 = get_store \<omega>2 \<and> r \<noteq> None then Some (Ag (get_store \<omega>1), the r)
+  else None))" (is "?A = ?B")
+proof (cases "\<omega>1 \<oplus> \<omega>2")
+  case None
+  then have "get_abs_state \<omega>1 \<oplus> get_abs_state \<omega>2 = None \<or> get_store \<omega>1 \<noteq> get_store \<omega>2"
+    by (metis comp_prod defined_def get_abs_state_def get_store_trace_comp)
+  then show ?thesis
+    using None by auto
+next
+  case (Some x)
+  then have asm0: "get_store \<omega>1 = get_store \<omega>2 \<and> get_abs_state \<omega>1 \<oplus> get_abs_state \<omega>2 \<noteq> None"
+    by (metis comp_prod defined_def get_store_trace_comp get_abs_state_def option.simps(3))
+  then obtain r where "Some r = get_abs_state \<omega>1 \<oplus> get_abs_state \<omega>2"
+    by force
+  moreover have "fst \<omega>1 \<oplus> fst \<omega>2 = Some (Ag (get_store \<omega>1))"
+    by (metis (no_types, opaque_lifting) agreement.exhaust_sel asm0 core_is_smaller fst_conv get_store_def get_store_trace_comp greater_def smaller_compatible_core)
+  ultimately show ?thesis
+    by (smt (z3) asm0 get_abs_state_def option.sel plus_prodIAlt)
+qed
+
+
+
+lemma full_core_def:
+  "|\<omega>| = (Ag (get_store \<omega>),  |get_abs_state \<omega>| )"
+  by (smt (verit) agreement.exhaust_sel core_def core_is_smaller fst_conv get_abs_state_def get_store_def option.discI plus_state_def snd_conv)
+
+
+lemma full_add_defined:
+  "\<omega>1 \<oplus> \<omega>2 \<noteq> None \<longleftrightarrow> ((get_abs_state \<omega>1) \<oplus> (get_abs_state \<omega>2) \<noteq> None \<and> get_store \<omega>1 = get_store \<omega>2)"
+  using plus_state_def[of \<omega>1 \<omega>2] option.discI
+  by (smt (verit, del_insts))
+
+lemma full_add_charact:
+  assumes "Some x = a \<oplus> b"
+  shows "get_store x = get_store a"
+      and "Some (get_abs_state x) = (get_abs_state a) \<oplus> (get_abs_state b)"
+proof -
+  show "get_store x = get_store a"
+    by (smt (verit) agreement.exhaust_sel assms fst_conv get_store_def option.discI option.sel plus_state_def)
+  show "Some (get_abs_state x) = (get_abs_state a) \<oplus> (get_abs_state b)" 
+    by (smt assms get_abs_state_def option.exhaust_sel option.sel option.simps(3) plus_state_def snd_conv)
+qed
+
+lemma full_state_ext:
+  assumes "get_store a = get_store b"
+      and "get_abs_state a = get_abs_state b"
+    shows "a = b"
+  by (metis agreement.exhaust_sel assms get_abs_state_def get_store_def prod_eqI)
+
+lemma add_defined_lift:
+  fixes s :: "'v ag_store"
+  assumes "Some c = a \<oplus> b"
+  shows "Some (s, c) = (s, a) \<oplus> (s, b)"
+proof -
+  have "Some s = s \<oplus> s"
+    by (simp add: plus_agreement_def)
+  then show ?thesis using plus_prodIAlt assms 
+    by fastforce
+qed
+
+lemma ag_store_greater:
+  fixes s :: "'v ag_store"
+  shows "s' \<succeq> s \<longleftrightarrow> s = s'"
+  by (metis ag_comp smaller_compatible_core succ_refl)
+
+lemma greater_charact:
+  "\<omega>' \<succeq> \<omega> \<longleftrightarrow> get_store \<omega> = get_store \<omega>' \<and> get_abs_state \<omega>' \<succeq> get_abs_state \<omega>" (is "?A \<longleftrightarrow> ?B")
+proof
+  show "?A \<Longrightarrow> ?B"
+    by (metis (no_types, opaque_lifting) get_abs_state_def get_store_trace_comp greater_prod_eq smaller_compatible)
+  assume ?B
+  then have "Ag (get_store \<omega>') \<succeq> Ag (get_store \<omega>) \<and> get_abs_state \<omega>' \<succeq> get_abs_state \<omega>"
+    by (simp add: succ_refl)
+  then show ?A
+    by (simp add: get_abs_state_def get_store_def greater_prod_eq)
+qed
+
+lemma core_charact:
+  shows "get_store |\<omega>| = get_store \<omega>"
+    and "get_abs_state |\<omega>| = |get_abs_state \<omega>|"
+   apply (simp add: full_core_def get_store_def)
+  by (simp add: full_core_def get_abs_state_def)
+
+
+
+
+
+
+
+
+
+
+
+
 
 section Start
 
-type_synonym 'a assertion = "'a \<Rightarrow> bool"
-
+type_synonym 'a assertion = "'a set"
 
 type_synonym 'a bexp = "'a \<rightharpoonup> bool"
 type_synonym ('a, 'v) exp = "'a \<rightharpoonup> 'v"
@@ -14,167 +181,194 @@ type_synonym 'v abs_vtyp = "'v set"
 text \<open>Types:
 - 'a: State (with ag_store, trace, heap...)
 - 'v: Type of values
-- 'r: Type of heap locations
+- 'r: Custom type
 \<close>
 
-datatype ('a, 'v, 'r) abs_stmt =
+datatype ('a, 'v, 'c) abs_stmt =
 
 \<comment>\<open>Assertions\<close>
   Inhale "'a assertion" | Exhale "'a assertion" | Assert "'a assertion" | Assume "'a assertion"
 
 \<comment>\<open>Control structures\<close>
-| If "'a bexp" "('a, 'v, 'r) abs_stmt" "('a, 'v, 'r) abs_stmt"
-| Seq "('a, 'v, 'r) abs_stmt" "('a, 'v, 'r) abs_stmt" (infixl ";;" 60)
+| If "'a bexp" "('a, 'v, 'c) abs_stmt" "('a, 'v, 'c) abs_stmt"
+| Seq "('a, 'v, 'c) abs_stmt" "('a, 'v, 'c) abs_stmt" (infixl ";;" 60)
 
 \<comment>\<open>Assignments\<close>
 | LocalAssign var "('a, 'v) exp"
 | Havoc var
+
+(*
 | FieldAssign "('a, 'r) exp" "('a, 'v) exp"
+(* TODO: Probably should be a parameter of the locale! *)
+*)
+| Custom 'c
 
-
+(*
 \<comment>\<open>Misc\<close>
-| Label label
-| Scope "'v abs_vtyp" "('a, 'v, 'r) abs_stmt"
+| Label label (* Should this one be a parameter of the locale as well? *)
+*)
+
+(*
+| Scope "'v abs_vtyp" "('a, 'v, 'c) abs_stmt"
+*)
 | Skip
 
-record ('v, 'r) abs_type_context =
+record ('v, 'c) abs_type_context =
   variables :: "var \<rightharpoonup> 'v abs_vtyp"
-  heap_locs :: "'r \<rightharpoonup> 'v abs_vtyp"
+  custom_context :: 'c
 
-(* Should also have a mapping from heap loc to abs_typ *)
-(*
-definition get_store :: "('v, 'a) abs_state \<Rightarrow> (var \<rightharpoonup> 'v)" where "get_store = the_ag \<circ> fst"
-*)
-
-locale semantics =
-
-  fixes has_value :: "('a :: sep_algebra) \<Rightarrow> 'r \<Rightarrow> 'v \<Rightarrow> bool"
-  fixes has_write_perm_only :: "'a \<Rightarrow> 'r \<Rightarrow> bool"
-  fixes set_value :: "'a \<Rightarrow> 'r \<Rightarrow> 'v \<Rightarrow> 'a"
-
-(* Axioms
-- TODO: Add smth about has_value
-*)
-  assumes frame_preserving_writing_orig: "Some x = a \<oplus> b \<Longrightarrow> stable b \<Longrightarrow> has_write_perm_only a hl \<Longrightarrow> Some (set_value x hl v) = set_value a hl v \<oplus> b"
-      and has_write_perm_only_same: "has_write_perm_only a hl \<Longrightarrow> has_write_perm_only b hl \<Longrightarrow> stabilize a = stabilize b"
-  (* TODO: WRONG! Needs something about the value! *)
-
-      and set_value_then_has_value: "has_write_perm_only a hl \<Longrightarrow> has_value (set_value a hl v) hl v"
-
-begin
-
-
-(* Needed:
-- Checking perm(x.f) = 1
-- Setting x.f := 5
-- Checking x.f = something
+(* Should also have a mapping from heap loc to abs_typ?
+Maybe should not...
  *)
 
-definition has_write_perm :: "'a \<Rightarrow> 'r \<Rightarrow> bool" where
-  "has_write_perm x hl \<longleftrightarrow> (\<exists>r. x \<succeq> r \<and> has_write_perm_only r hl)"
+locale typed_state =
+    fixes wf_custom_state :: "'c \<Rightarrow> ('a :: sep_algebra) \<Rightarrow> bool"
+  assumes wf_custom_state_sum: "Some x = a \<oplus> b \<Longrightarrow> wf_custom_state \<Gamma> a \<Longrightarrow> wf_custom_state \<Gamma> b \<Longrightarrow> wf_custom_state \<Gamma> x"
+      and wf_custom_state_smaller: "a \<succeq> b \<Longrightarrow> wf_custom_state \<Gamma> a \<Longrightarrow> wf_custom_state \<Gamma> b"
+      and wf_custom_state_core_aux: "wf_custom_state \<Gamma> |x| \<Longrightarrow> wf_custom_state \<Gamma> x"
+begin
 
-definition inh ("\<langle>_\<rangle>" [51] 81) where
-  "\<langle>A\<rangle> = { \<omega> |\<omega>. A \<omega> }"
+definition typed_store :: "('v, 'c) abs_type_context \<Rightarrow> (var \<rightharpoonup> 'v) \<Rightarrow> bool" where
+  "typed_store \<Delta> \<sigma> \<longleftrightarrow> (dom (variables \<Delta>) = dom \<sigma> \<and> (\<forall>x v ty. \<sigma> x = Some v \<and> variables \<Delta> x = Some ty \<longrightarrow> v \<in> ty))"
+
+
+lemma typed_storeI:
+  assumes "dom (variables \<Delta>) = dom \<sigma>"
+      and "\<And>x v ty. \<sigma> x = Some v \<Longrightarrow> variables \<Delta> x = Some ty \<Longrightarrow> v \<in> ty"
+    shows "typed_store \<Delta> \<sigma>"
+  using assms(1) assms(2) typed_store_def by meson
+
+lemma wf_custom_state_core: "wf_custom_state \<Gamma> |x| \<longleftrightarrow> wf_custom_state \<Gamma> x"
+  using max_projection_prop_pure_core mpp_smaller wf_custom_state_core_aux wf_custom_state_smaller by blast
+
+
+
+definition typed_exp where
+  "typed_exp ty e \<longleftrightarrow> (\<forall>\<omega> v. e \<omega> = Some v \<longrightarrow> v \<in> ty)"
 
 definition filter_dom where
   "filter_dom vars S = Set.filter (\<lambda>\<omega>. dom (get_store \<omega>) = vars) S"
 
-definition self_framing :: "(('v, 'a) abs_state \<Rightarrow> bool) \<Rightarrow> bool" where
-  "self_framing A \<longleftrightarrow> (\<forall>\<omega>. A \<omega> \<longleftrightarrow> A (stabilize \<omega>))"
+subsection \<open>Typed stuff\<close>
+
+subsection \<open>States\<close>
+
+definition typed where
+  "typed \<Delta> \<omega> \<longleftrightarrow> typed_store \<Delta> (get_store \<omega>) \<and> wf_custom_state (custom_context \<Delta>) (get_abs_state \<omega>)"
+
+definition self_framing_typed where
+  "self_framing_typed \<Delta> A \<longleftrightarrow> (\<forall>\<omega>. typed \<Delta> \<omega> \<longrightarrow> (\<omega> \<in> A \<longleftrightarrow> stabilize \<omega> \<in> A))"
+
+lemma self_framing_typedI:
+  assumes "\<And>\<omega>. typed \<Delta> \<omega> \<Longrightarrow> (\<omega> \<in> A \<longleftrightarrow> stabilize \<omega> \<in> A)"
+  shows "self_framing_typed \<Delta> A"
+  using assms self_framing_typed_def by blast
+
+definition wf_state where
+  "wf_state \<Delta> \<omega> \<longleftrightarrow> (stable \<omega> \<and> typed \<Delta> \<omega>)"
+
+definition Stabilize_typed where
+  "Stabilize_typed \<Delta> A = Set.filter (typed \<Delta>) (Stabilize A)"
 
 
-text \<open>The truth of A in a only depends on parts of a (for a ## \<omega>) that:
-1) are stable, or
-2) are given by |\<omega>|\<close>
-definition rel_stable_assertion where
-(*  "rel_stable_assertion \<omega> A \<longleftrightarrow> (\<forall>\<omega>'. \<omega> ## \<omega>' \<longrightarrow> (A \<omega>' \<longleftrightarrow> A (stabilize_rel \<omega> \<omega>')))" *)
-(*  "rel_stable_assertion \<omega> A \<longleftrightarrow> (\<forall>x a. \<omega> ## a \<and> pure_larger x (stabilize a) \<and> x \<succeq> |\<omega>| \<longrightarrow> (A a \<longleftrightarrow> A x))" *)
-  "rel_stable_assertion \<omega> A \<longleftrightarrow> Stable ({\<omega>} \<otimes> \<langle>A\<rangle>)"
+lemma typed_then_stabilize_typed:
+  assumes "typed \<Delta> \<omega>"
+  shows "typed \<Delta> (stabilize \<omega>)"
+  by (metis (no_types, lifting) assms greater_charact max_projection_prop_def max_projection_prop_stable_stabilize typed_def wf_custom_state_smaller)
 
-section \<open>Operational semantics\<close>
+lemma self_framing_Stabilize_typed[simp]:
+  "self_framing_typed \<Delta> (Stabilize_typed \<Delta> A)"
+proof (rule self_framing_typedI)
+  fix \<omega>
+  assume asm0: "typed \<Delta> \<omega>"
+  then show "(\<omega> \<in> Stabilize_typed \<Delta> A) = (stabilize \<omega> \<in> Stabilize_typed \<Delta> A)"
+    by (simp add: Stabilize_typed_def already_stable typed_then_stabilize_typed)
+qed
 
-inductive red_stmt :: "('v, 'r) abs_type_context \<Rightarrow> (('v, 'a) abs_state, 'v, 'r) abs_stmt \<Rightarrow> ('v, 'a) abs_state \<Rightarrow> ('v, 'a) abs_state set \<Rightarrow> bool"
-  and sequential_composition :: "('v, 'r) abs_type_context \<Rightarrow> ('v, 'a) abs_state set \<Rightarrow> (('v, 'a) abs_state, 'v, 'r) abs_stmt \<Rightarrow> ('v, 'a) abs_state set \<Rightarrow> bool"
-where
+lemma typed_state_then_stabilize_typed:
+  assumes "typed \<Delta> \<omega>"
+  shows "typed \<Delta> (stabilize \<omega>)"
+  by (smt (verit, best) assms greater_charact max_projection_prop_stable_stabilize mpp_smaller typed_def wf_custom_state_smaller)
 
-\<comment>\<open>f maps each x to one possible final set of states: It performs the angelic choice\<close>
-  SeqComp: "\<lbrakk> \<And>\<omega>. \<omega> \<in> S \<Longrightarrow> (red_stmt \<Delta> C \<omega> (f \<omega>)) ; S' = Union (f ` S) \<rbrakk> \<Longrightarrow> sequential_composition \<Delta> S C S'"
+lemma typed_sum:
+  assumes "Some x = a \<oplus> b"
+      and "typed \<Delta> a"
+      and "typed \<Delta> b"
+    shows "typed \<Delta> x"
+  by (smt (verit, del_insts) assms(1) assms(2) assms(3) full_add_charact(1) full_add_charact(2) typed_def wf_custom_state_sum)
 
-| RedSkip: "red_stmt \<Delta> Skip \<omega> ({\<omega>})"
+lemma typed_core:
+  assumes "typed \<Delta> a"
+  shows "typed \<Delta> |a|"
+  by (metis assms core_charact(1) core_charact(2) typed_def wf_custom_state_core)
 
-| RedAssertTrue: "\<lbrakk> A \<omega> \<rbrakk> \<Longrightarrow> red_stmt \<Delta> (Assert A) \<omega> ({\<omega>})"
-| RedAssumeTrue: "\<lbrakk> rel_stable_assertion \<omega> A; A \<omega> \<rbrakk> \<Longrightarrow> red_stmt \<Delta> (Assume A) \<omega> ({\<omega>})"
-| RedAssumeFalse: "\<lbrakk> rel_stable_assertion \<omega> A; \<not> A \<omega> \<rbrakk> \<Longrightarrow> red_stmt \<Delta> (Assume A) \<omega> ({})"
+lemma typed_smaller:
+  assumes "typed \<Delta> \<omega>'"
+      and "\<omega>' \<succeq> \<omega>"
+    shows "typed \<Delta> \<omega>"
+  by (metis assms(1) assms(2) greater_charact typed_def wf_custom_state_smaller)
+
+subsection \<open>Assertions\<close>
+
+definition typed_assertion where
+  "typed_assertion \<Delta> A \<longleftrightarrow> (\<forall>\<omega>\<in>A. typed \<Delta> \<omega>)"
+
+lemma typed_assertionI:
+  assumes "\<And>\<omega>. \<omega> \<in> A \<Longrightarrow> typed \<Delta> \<omega>"
+  shows "typed_assertion \<Delta> A"
+  using assms typed_assertion_def by blast
+
+lemma typed_assertionE:
+  assumes "typed_assertion \<Delta> A"
+      and "\<omega> \<in> A"
+    shows "typed \<Delta> \<omega>"
+  using assms typed_assertion_def by blast
+
+lemma typed_subset:
+  assumes "A \<subseteq> A'"
+      and "typed_assertion \<Delta> A'"
+    shows "typed_assertion \<Delta> A"
+  using assms(1) assms(2) typed_assertion_def by blast
+
+lemma typed_star:
+  assumes "typed_assertion \<Delta> A"
+      and "typed_assertion \<Delta> B"
+    shows "typed_assertion \<Delta> (A \<otimes> B)"
+  by (meson assms(1) assms(2) typed_assertion_def typed_sum x_elem_set_product)
 
 
 
-| RedInhale: "\<lbrakk> rel_stable_assertion \<omega> A \<rbrakk> \<Longrightarrow> red_stmt \<Delta> (Inhale A) \<omega> (Set.filter stable ({\<omega>} \<otimes> \<langle>A\<rangle>))"
-| RedExhale: "\<lbrakk> a \<in> \<langle>A\<rangle> ; Some \<omega> = \<omega>' \<oplus> a ; stable \<omega>' \<rbrakk> \<Longrightarrow> red_stmt \<Delta> (Exhale A) \<omega> {\<omega>'}"
+lemma typed_Stabilize_typed[simp]:
+  "typed_assertion \<Delta> (Stabilize_typed \<Delta> A)"
+  by (simp add: Stabilize_typed_def typed_assertion_def)
 
-| RedIfTrue: "\<lbrakk> b \<omega> = Some True ; red_stmt \<Delta> C1 \<omega> S \<rbrakk> \<Longrightarrow> red_stmt \<Delta> (If b C1 C2) \<omega> S"
-| RedIfFalse: "\<lbrakk> b \<omega> = Some False ; red_stmt \<Delta> C2 \<omega> S \<rbrakk> \<Longrightarrow> red_stmt \<Delta> (If b C1 C2) \<omega> S"
+lemma self_framing_typed_on_typed:
+  assumes "self_framing_typed \<Delta> P"
+      and "typed_assertion \<Delta> A"
+    shows "self_framing_on A P"
+by (meson assms(1) assms(2) self_framing_on_def self_framing_typed_def typed_assertion_def)
 
-| RedSeq: "\<lbrakk> red_stmt \<Delta> C1 \<omega> S1 ; sequential_composition \<Delta> S1 C2 S2 \<rbrakk> \<Longrightarrow> red_stmt \<Delta> (C1 ;; C2) \<omega> S2"
+definition wf_set where
+  "wf_set \<Delta> S \<longleftrightarrow> (\<forall>x \<in> S. wf_state \<Delta> x)"
 
-\<comment>\<open>No need to handle the case where the variable is not defined, since it is part of well-definedness of a program\<close>
-| RedLocalAssign: "\<lbrakk>variables \<Delta> x = Some ty; e \<omega> = Some v; v \<in> ty \<rbrakk> \<Longrightarrow>
-   red_stmt \<Delta> (LocalAssign x e) \<omega> ({set_store \<omega> ((get_store \<omega>)(x := Some v)) })"
+definition assign_var_state :: "var \<Rightarrow> 'v option \<Rightarrow> ('v, 'a) abs_state \<Rightarrow> ('v, 'a) abs_state" where
+  "assign_var_state x v \<omega> = set_store \<omega> ((get_store \<omega>)(x := v))"
 
+lemma assign_var_state_stable:
+  "stable \<omega> \<longleftrightarrow> stable (assign_var_state x v \<omega>)"
+  by (metis (no_types, lifting) already_stable assign_var_state_def full_state_ext get_abs_state_set_store get_store_stabilize set_store_stabilize stabilize_is_stable)
 
-| RedHavoc: "variables \<Delta> x = Some ty \<Longrightarrow>
-  red_stmt \<Delta> (Havoc x) \<omega> ({set_store \<omega> ((get_store \<omega>)(x := Some v)) |v. v \<in> ty})"
+lemma assign_var_state_stabilize:
+  "stabilize (assign_var_state x v \<omega>) = assign_var_state x v (stabilize \<omega>)"
+  by (simp add: assign_var_state_def)
 
-| RedFieldAssign: "\<lbrakk> r \<omega> = Some hl ; e \<omega> = Some v ; has_write_perm (get_state \<omega>) hl; heap_locs \<Delta> hl = Some ty; v \<in> ty \<rbrakk>
-  \<Longrightarrow> red_stmt \<Delta> (FieldAssign r e) \<omega> {set_state \<omega> (set_value (get_state \<omega>) hl v)}"
-
-| RedLabel: "red_stmt \<Delta> (Label l) \<omega> {set_trace \<omega> ((get_trace \<omega>)(l:= Some (get_state \<omega>)))}"
-
-
-(*
-
-\<comment>\<open>Updated type context\<close>
-| RedScope: "\<lbrakk> sequential_composition Pr (shift_and_add_list T tys) E { (\<sigma>', \<tau>, \<phi>) |\<sigma>'. \<sigma>' \<in> declare_var_list (domains \<Delta>) tys \<sigma>} s r \<rbrakk> \<Longrightarrow>
-  red_stmt \<Delta> (Scope ty s) (\<sigma>, \<tau>, \<phi>) ((unshift_state 1 ` r))"
-*)
-
-
-(*
-
-(* Only rets and args defined when executing a method call, also empty trace *)
-(* If method does not exist, or wrong number of args or rets: Not well-defined *)
-(* Concrete method *)
-
-(* r is the "frame" *)
-
-(* Two things to verify:
-- exhale I ; havoc l ; inhale I ; assume not(b)
-- havoc l ; assume b ; inhale I ; s \<longrightarrow> satisfies I
-*)
-
-Needs type context to havoc
-*)
-
-definition typed_store :: "('v, 'r) abs_type_context \<Rightarrow> (var \<rightharpoonup> 'v) \<Rightarrow> bool" where
-  "typed_store \<Delta> \<sigma> \<longleftrightarrow> (dom (variables \<Delta>) = dom \<sigma> \<and> (\<forall>x v ty. \<sigma> x = Some v \<and> variables \<Delta> x = Some ty \<longrightarrow> v \<in> ty))"
-
-section \<open>Assertions\<close>
-
-subsection \<open>General concepts\<close>
-
-definition framed_by :: "('v, 'a) abs_state assertion \<Rightarrow> ('v, 'a) abs_state assertion \<Rightarrow> bool" where
-  "framed_by A B \<longleftrightarrow> (\<forall>\<omega> \<in> \<langle>A\<rangle>. stable \<omega> \<longrightarrow> rel_stable_assertion \<omega> B)"
-
-definition wf_exp where
-  "wf_exp e \<longleftrightarrow> (\<forall>a b v. a \<succeq> b \<and> e b = Some v \<longrightarrow> e a = Some v) \<and> (\<forall>a. e a = e |a| )"
-
-definition framed_by_exp where
-  "framed_by_exp A e \<longleftrightarrow> (\<forall>\<omega> \<in> \<langle>A\<rangle>. e \<omega> \<noteq> None)"
-
-definition entails where
-  "entails A B \<longleftrightarrow> \<langle>A\<rangle> \<subseteq> \<langle>B\<rangle>"
-
-definition equiv where
-  "equiv A B \<longleftrightarrow> \<langle>A\<rangle> = \<langle>B\<rangle>"
+lemma typed_assign_var:
+  assumes "typed \<Delta> \<omega>"
+      and "variables \<Delta> x = Some ty"
+      and "v \<in> ty"
+    shows "typed \<Delta> (assign_var_state x (Some v) \<omega>)"
+  using assms unfolding  assign_var_state_def typed_def
+  by (smt (verit, del_insts) dom_fun_upd get_abs_state_set_store get_store_set_store insert_dom map_upd_Some_unfold option.discI typed_store_def)
 
 
 
@@ -183,8 +377,8 @@ section \<open>Free variables\<close>
 definition equal_on_set :: "var set \<Rightarrow> (var \<rightharpoonup> 'v) \<Rightarrow> (var \<rightharpoonup> 'v) \<Rightarrow> bool" where
   "equal_on_set S \<sigma>1 \<sigma>2 \<longleftrightarrow> (\<forall>x \<in> S. \<sigma>1 x = \<sigma>2 x)"
 
-definition overapprox_fv :: "('v, 'r) abs_type_context \<Rightarrow> ('v, 'a) abs_state assertion \<Rightarrow> var set \<Rightarrow> bool" where
-  "overapprox_fv \<Delta> A S \<longleftrightarrow> (\<forall>\<sigma>1 \<sigma>2 \<tau> \<gamma>. typed_store \<Delta> \<sigma>1 \<and> typed_store \<Delta> \<sigma>2 \<and> equal_on_set S \<sigma>1 \<sigma>2 \<longrightarrow> (A ((Ag \<sigma>1, \<tau>), \<gamma>) \<longleftrightarrow> A ((Ag \<sigma>2, \<tau>), \<gamma>)))"
+definition overapprox_fv :: "('v, 'c) abs_type_context \<Rightarrow> ('v, 'a) abs_state assertion \<Rightarrow> var set \<Rightarrow> bool" where
+  "overapprox_fv \<Delta> A S \<longleftrightarrow> (\<forall>\<sigma>1 \<sigma>2 \<gamma>. typed_store \<Delta> \<sigma>1 \<and> typed_store \<Delta> \<sigma>2 \<and> equal_on_set S \<sigma>1 \<sigma>2 \<longrightarrow> ((Ag \<sigma>1, \<gamma>) \<in> A \<longleftrightarrow> (Ag \<sigma>2, \<gamma>) \<in> A))"
 
 
 definition free_vars where
@@ -197,24 +391,190 @@ definition at_least_two_elems:
 
 subsection \<open>wf_assertion\<close>
 
-(* TODO: Is it needed? *)
-definition wf_assertion :: "('v, 'a) abs_state assertion \<Rightarrow> bool" where
-  "wf_assertion A \<longleftrightarrow> (\<forall>x' x. pure_larger x' x \<and> A x \<longrightarrow> A x')"
+definition wf_assertion :: "('v, 'c) abs_type_context \<Rightarrow> ('v, 'a) abs_state assertion \<Rightarrow> bool" where
+  "wf_assertion \<Delta> A \<longleftrightarrow> typed_assertion \<Delta> A \<and> (\<forall>x' x. pure_larger x' x \<and> typed \<Delta> x' \<and> x \<in> A \<longrightarrow> x' \<in> A)"
+
+lemma wf_assertionE:
+  assumes "wf_assertion \<Delta> A"
+      and "pure_larger x' x"
+      and "typed \<Delta> x'"
+      and "x \<in> A"
+    shows "x' \<in> A"
+  using assms(1) assms(2) assms(3) assms(4) typed_state.wf_assertion_def typed_state_axioms by blast
+
+(*
+lemma self_framing_wfI:
+  assumes "wf_assertion \<Delta> A"
+      and "\<And>\<omega>. \<omega> \<in> A \<Longrightarrow> stabilize \<omega> \<in> A"
+    shows "self_framing A"
+  unfolding self_framing_def
+proof -
+  have "\<And>\<omega>. stabilize \<omega> \<in> A \<Longrightarrow> \<omega> \<in> A"
+  proof -
+    fix \<omega> assume "stabilize \<omega> \<in> A"
+    then have "pure_larger \<omega> (stabilize \<omega>)"
+      using core_is_pure decompose_stabilize_pure pure_def pure_larger_def by blast
+    then show "\<omega> \<in> A"
+      using \<open>stabilize \<omega> \<in> A\<close> assms(1) wf_assertion_def by blast
+  qed
+  then show "\<forall>\<omega>. (\<omega> \<in> A) = (stabilize \<omega> \<in> A)" using assms(2) by blast
+qed
+*)
+
+definition exists_assert :: "('v, 'c) abs_type_context \<Rightarrow> var \<Rightarrow> ('v, 'a) abs_state assertion \<Rightarrow> ('v, 'a) abs_state assertion" where
+  "exists_assert \<Delta> x A =
+{ \<omega> |\<omega> v0 v ty. typed \<Delta> \<omega> \<and> v0 \<in> ty \<and> get_store \<omega> x = Some v0 \<and> variables \<Delta> x = Some ty \<and> v \<in> ty \<and> assign_var_state x (Some v) \<omega> \<in> A}"
 
 
-fun wf_abs_stmt where
-  "wf_abs_stmt \<Delta> Skip \<longleftrightarrow> True"
-| "wf_abs_stmt \<Delta> (Inhale A) \<longleftrightarrow> wf_assertion A"
-| "wf_abs_stmt \<Delta> (Exhale A) \<longleftrightarrow> wf_assertion A"
-| "wf_abs_stmt \<Delta> (Assert A) \<longleftrightarrow> wf_assertion A"
-| "wf_abs_stmt \<Delta> (Assume A) \<longleftrightarrow> wf_assertion A"
-| "wf_abs_stmt \<Delta> (If b C1 C2) \<longleftrightarrow> wf_exp b \<and> wf_abs_stmt \<Delta> C1 \<and> wf_abs_stmt \<Delta> C2"
-| "wf_abs_stmt \<Delta> (Seq C1 C2) \<longleftrightarrow> wf_abs_stmt \<Delta> C1 \<and> wf_abs_stmt \<Delta> C2"
-| "wf_abs_stmt \<Delta> (LocalAssign x e) \<longleftrightarrow> wf_exp e"
-| "wf_abs_stmt \<Delta> (FieldAssign r e) \<longleftrightarrow> wf_exp r \<and> wf_exp e"
-| "wf_abs_stmt \<Delta> (Havoc x) \<longleftrightarrow> x \<in> dom (variables \<Delta>)"
-| "wf_abs_stmt \<Delta> (Label _) \<longleftrightarrow> True" (* TODO: Prevent duplicate labels? *)
-| "wf_abs_stmt \<Delta> (Scope _ C) \<longleftrightarrow> wf_abs_stmt \<Delta> C" (* TODO: Prevent duplicate labels? *)
+
+lemma self_framing_typedE:
+  assumes "self_framing_typed \<Delta> A"
+      and "typed \<Delta> a"
+      and "a \<in> A"
+    shows "stabilize a \<in> A"
+  using assms(1) assms(2) assms(3) self_framing_typed_def by blast
+
+lemma self_framing_typed_altE:
+  assumes "self_framing_typed \<Delta> A"
+      and "typed \<Delta> a"
+      and "stabilize a \<in> A"
+    shows "a \<in> A"
+  using assms(1) assms(2) assms(3) self_framing_typed_def by blast
+
+
+lemma self_framing_typed_ext:
+  assumes "self_framing_typed \<Delta> A"
+      and "self_framing_typed \<Delta> B"
+      and "typed_assertion \<Delta> A"
+      and "typed_assertion \<Delta> B"
+      and "\<And>\<omega>. stable \<omega> \<Longrightarrow> typed \<Delta> \<omega> \<Longrightarrow> \<omega> \<in> A \<Longrightarrow> \<omega> \<in> B"
+      and "\<And>\<omega>. stable \<omega> \<Longrightarrow> typed \<Delta> \<omega>  \<Longrightarrow> \<omega> \<in> B \<Longrightarrow> \<omega> \<in> A"
+    shows "A = B"
+proof -
+  have "\<And>\<omega>. \<omega> \<in> A \<longleftrightarrow> \<omega> \<in> B"
+    by (meson assms(1) assms(2) assms(3) assms(4) assms(5) assms(6) self_framing_typedE self_framing_typed_altE typed_assertion_def stabilize_is_stable)
+  then show ?thesis by blast
+qed
+
+
+
+lemma wf_exp_framed_by_stabilize_typed:
+  assumes "wf_exp e"
+      and "framed_by_exp A e"
+      and "\<omega> \<in> A"
+      and "typed \<Delta> \<omega>"
+      and "self_framing_typed \<Delta> A"
+    shows "e \<omega> = Some b \<longleftrightarrow> e (stabilize \<omega>) = Some b"
+proof
+  show "e (stabilize \<omega>) = Some b \<Longrightarrow> e \<omega> = Some b"
+    by (metis (no_types, lifting) assms(1) max_projection_prop_def max_projection_prop_stable_stabilize wf_expE)
+  assume "e \<omega> = Some b"
+  moreover obtain v where "e (stabilize \<omega>) = Some v"
+    by (metis assms(2) assms(3) assms(4) assms(5) framed_by_expE self_framing_typedE)
+  ultimately show "e (stabilize \<omega>) = Some b"
+    by (metis (mono_tags, lifting) assms(1) max_projection_prop_def max_projection_prop_stable_stabilize wf_expE)
+qed
+
+
+end
+
+
+
+
+
+
+
+section \<open>Semantics\<close>
+
+locale semantics =
+  typed_state wf_custom_state for wf_custom_state :: "'c \<Rightarrow> ('a :: sep_algebra) \<Rightarrow> bool" +
+  
+  fixes red_custom_stmt :: "('v, 'c) abs_type_context \<Rightarrow> 's \<Rightarrow> ('v, 'a) abs_state \<Rightarrow> ('v, 'a) abs_state set \<Rightarrow> bool"
+  fixes wf_custom_stmt :: "('v, 'c) abs_type_context \<Rightarrow> 's \<Rightarrow> bool"
+  fixes SL_Custom :: "('v, 'c) abs_type_context \<Rightarrow> ('v, 'a) abs_state set \<Rightarrow> 's \<Rightarrow> ('v, 'a) abs_state set \<Rightarrow> bool"
+
+  assumes SL_proof_custom: "(\<forall>(\<omega> :: (('v, 'a) abs_state list \<times> ('v, 'a) abs_state)) \<in> SA.
+  red_custom_stmt \<Delta> C (snd \<omega>) (f \<omega>)) \<Longrightarrow> wf_custom_stmt \<Delta> C \<Longrightarrow> wf_set \<Delta> (snd ` SA)
+  \<Longrightarrow> SL_Custom \<Delta> (Stabilize_typed \<Delta> (snd ` SA)) C (Stabilize_typed \<Delta> (\<Union>\<omega>\<in>SA. f \<omega>))"
+
+      and red_custom_stable: "red_custom_stmt \<Delta> C \<omega> S \<Longrightarrow> stable \<omega> \<Longrightarrow> \<omega>' \<in> S \<Longrightarrow> stable \<omega>'"
+      and red_custom_typed_store: "red_custom_stmt \<Delta> C \<omega> S \<Longrightarrow> typed_store \<Delta> (get_store \<omega>)
+  \<Longrightarrow> \<omega>' \<in> S \<Longrightarrow> typed_store \<Delta> (get_store \<omega>')"
+
+      and red_wf_custom: "red_custom_stmt \<Delta> C \<omega> S \<Longrightarrow> wf_custom_state (custom_context \<Delta>) (get_abs_state \<omega>) \<Longrightarrow>
+        wf_custom_stmt \<Delta> C \<Longrightarrow> \<omega>' \<in> S \<Longrightarrow> wf_custom_state (custom_context \<Delta>) (get_abs_state \<omega>')"
+
+      and red_wf_complete: "SL_Custom \<Delta> A C B \<Longrightarrow> \<omega> \<in> A \<Longrightarrow> wf_custom_stmt \<Delta> C \<Longrightarrow> stable \<omega>
+          \<Longrightarrow> typed \<Delta> \<omega> \<Longrightarrow> (\<exists>S. red_custom_stmt \<Delta> C \<omega> S \<and> S \<subseteq> B)"
+
+begin
+
+section \<open>Operational semantics\<close>
+
+inductive red_stmt :: "('v, 'c) abs_type_context \<Rightarrow> (('v, 'a) abs_state, 'v, 's) abs_stmt \<Rightarrow> ('v, 'a) abs_state \<Rightarrow> ('v, 'a) abs_state set \<Rightarrow> bool"
+  and sequential_composition :: "('v, 'c) abs_type_context \<Rightarrow> ('v, 'a) abs_state set \<Rightarrow> (('v, 'a) abs_state, 'v, 's) abs_stmt \<Rightarrow> ('v, 'a) abs_state set \<Rightarrow> bool"
+where
+
+\<comment>\<open>f maps each x to one possible final set of states: It performs the angelic choice\<close>
+  SeqComp: "\<lbrakk> \<And>\<omega>. \<omega> \<in> S \<Longrightarrow> (red_stmt \<Delta> C \<omega> (f \<omega>)) ; S' = Union (f ` S) \<rbrakk> \<Longrightarrow> sequential_composition \<Delta> S C S'"
+
+| RedSkip: "red_stmt \<Delta> Skip \<omega> ({\<omega>})"
+
+| RedAssertTrue: "\<lbrakk> \<omega> \<in> A \<rbrakk> \<Longrightarrow> red_stmt \<Delta> (Assert A) \<omega> ({\<omega>})"
+| RedAssumeTrue: "\<lbrakk> stable_on \<omega> A; \<omega> \<in> A \<rbrakk> \<Longrightarrow> red_stmt \<Delta> (Assume A) \<omega> ({\<omega>})"
+| RedAssumeFalse: "\<lbrakk> stable_on \<omega> A; \<omega> \<notin> A \<rbrakk> \<Longrightarrow> red_stmt \<Delta> (Assume A) \<omega> ({})"
+
+| RedInhale: "\<lbrakk> rel_stable_assertion \<omega> A \<rbrakk> \<Longrightarrow> red_stmt \<Delta> (Inhale A) \<omega> (Set.filter stable ({\<omega>} \<otimes> A))"
+| RedExhale: "\<lbrakk> a \<in> A ; Some \<omega> = \<omega>' \<oplus> a ; stable \<omega>' \<rbrakk> \<Longrightarrow> red_stmt \<Delta> (Exhale A) \<omega> {\<omega>'}"
+\<comment>\<open>Both Inhale and Exhale could be defined equivalently with stabilize instead of stable\<close>
+
+| RedIfTrue: "\<lbrakk> b \<omega> = Some True ; red_stmt \<Delta> C1 \<omega> S \<rbrakk> \<Longrightarrow> red_stmt \<Delta> (If b C1 C2) \<omega> S"
+| RedIfFalse: "\<lbrakk> b \<omega> = Some False ; red_stmt \<Delta> C2 \<omega> S \<rbrakk> \<Longrightarrow> red_stmt \<Delta> (If b C1 C2) \<omega> S"
+
+| RedSeq: "\<lbrakk> red_stmt \<Delta> C1 \<omega> S1 ; sequential_composition \<Delta> S1 C2 S2 \<rbrakk> \<Longrightarrow> red_stmt \<Delta> (C1 ;; C2) \<omega> S2"
+
+\<comment>\<open>No need to handle the case where the variable is not defined, since it is part of well-definedness of a program\<close>
+| RedLocalAssign: "\<lbrakk>variables \<Delta> x = Some ty; e \<omega> = Some v; v \<in> ty \<rbrakk> \<Longrightarrow>
+   red_stmt \<Delta> (LocalAssign x e) \<omega> ({assign_var_state x (Some v) \<omega>})"
+
+| RedHavoc: "variables \<Delta> x = Some ty \<Longrightarrow>
+  red_stmt \<Delta> (Havoc x) \<omega> ({ assign_var_state x (Some v) \<omega> |v. v \<in> ty})"
+
+| RedCustom: "red_custom_stmt \<Delta> C \<omega> S \<Longrightarrow> red_stmt \<Delta> (Custom C) \<omega> S"
+
+(*
+\<comment>\<open>Updated type context\<close>
+| RedScope: "\<lbrakk> variables \<Delta> x = None; \<Delta>' = \<Delta>\<lparr> variables := (variables \<Delta>)(x \<mapsto> ty) \<rparr>;
+sequential_composition \<Delta> { assign_var_state x (Some v) \<omega> |v. v \<in> ty } C S' \<rbrakk>
+\<Longrightarrow> red_stmt \<Delta> (Scope ty s) \<omega> {assign_var_state x None \<omega> |\<omega>. \<omega> \<in> S'}"
+*)
+
+
+
+
+
+inductive_cases sequential_composition_elim[elim!]: "sequential_composition \<Delta> S C S'"
+inductive_cases red_stmt_Seq_elim[elim!]: "red_stmt \<Delta> (Seq C1 C2) \<omega> S"
+inductive_cases red_stmt_Inhale_elim[elim!]: "red_stmt \<Delta> (Inhale A) \<omega> S"
+inductive_cases red_stmt_Exhale_elim[elim!]: "red_stmt \<Delta> (Exhale A) \<omega> S"
+inductive_cases red_stmt_Skip_elim[elim!]: "red_stmt \<Delta> Skip \<omega> S"
+inductive_cases red_stmt_Havoc_elim[elim!]: "red_stmt \<Delta> (Havoc x) \<omega> S"
+inductive_cases red_stmt_Assign_elim[elim!]: "red_stmt \<Delta> (LocalAssign x e) \<omega> S"
+inductive_cases red_stmt_If_elim[elim!]: "red_stmt \<Delta> (If b C1 C2) \<omega> S"
+inductive_cases red_stmt_Assert_elim[elim!]: "red_stmt \<Delta> (Assert A) \<omega> S"
+inductive_cases red_stmt_Assume_elim[elim!]: "red_stmt \<Delta> (Assume A) \<omega> S"
+(*
+inductive_cases red_stmt_FieldAssign_elim[elim!]: "red_stmt \<Delta> (FieldAssign l e) \<omega> S"
+*)
+inductive_cases red_stmt_Custom_elim[elim!]: "red_stmt \<Delta> (Custom C) \<omega> S"
+
+
+
+
+
+section \<open>Assertions\<close>
+
+subsection \<open>General concepts\<close>
 
 
 fun modif where
@@ -222,8 +582,19 @@ fun modif where
 | "modif (Havoc x) = {x}"
 | "modif (Seq C1 C2) = modif C1 \<union> modif C2"
 | "modif (If _ C1 C2) = modif C1 \<union> modif C2"
-| "modif (Scope _ C) = (\<lambda>x. x - 1) ` (Set.filter (\<lambda>x. x > 0) (modif C))" (* Shifting by one *)
 | "modif _ = {}"
+
+fun wf_abs_stmt where
+  "wf_abs_stmt \<Delta> Skip \<longleftrightarrow> True"
+| "wf_abs_stmt \<Delta> (Inhale A) \<longleftrightarrow> wf_assertion \<Delta> A"
+| "wf_abs_stmt \<Delta> (Exhale A) \<longleftrightarrow> wf_assertion \<Delta> A"
+| "wf_abs_stmt \<Delta> (Assert A) \<longleftrightarrow> wf_assertion \<Delta> A"
+| "wf_abs_stmt \<Delta> (Assume A) \<longleftrightarrow> wf_assertion \<Delta> A"
+| "wf_abs_stmt \<Delta> (If b C1 C2) \<longleftrightarrow> wf_exp b \<and> wf_abs_stmt \<Delta> C1 \<and> wf_abs_stmt \<Delta> C2"
+| "wf_abs_stmt \<Delta> (Seq C1 C2) \<longleftrightarrow> wf_abs_stmt \<Delta> C1 \<and> wf_abs_stmt \<Delta> C2"
+| "wf_abs_stmt \<Delta> (LocalAssign x e) \<longleftrightarrow> wf_exp e \<and> (\<exists>ty. variables \<Delta> x = Some ty \<and> typed_exp ty e)"
+| "wf_abs_stmt \<Delta> (Havoc x) \<longleftrightarrow> x \<in> dom (variables \<Delta>)"
+| "wf_abs_stmt \<Delta> (Custom C) \<longleftrightarrow> wf_custom_stmt \<Delta> C"
 
 fun havoc_list where
   "havoc_list [] = Skip"
@@ -232,12 +603,7 @@ fun havoc_list where
 
 subsection \<open>Assertion connectives\<close>
 
-definition pure_assertify where
-  "pure_assertify b \<omega> \<longleftrightarrow> b \<omega> = Some True"
-
-definition negate where
-  "negate b \<omega> = (if b \<omega> = None then None else Some (\<not> (the (b \<omega>))))"
-
+(*
 definition astar :: "('v, 'a) abs_state assertion \<Rightarrow> ('v, 'a) abs_state assertion \<Rightarrow> ('v, 'a) abs_state assertion"
  (infixl "&&" 60)
   where
@@ -251,21 +617,21 @@ definition aconj :: "('v, 'a) abs_state assertion \<Rightarrow> ('v, 'a) abs_sta
 
 definition adisj :: "('v, 'a) abs_state assertion \<Rightarrow> ('v, 'a) abs_state assertion \<Rightarrow> ('v, 'a) abs_state assertion"
  (infixl "||" 60) where "(A || B) \<omega> \<longleftrightarrow> A \<omega> \<or> B \<omega>"
+*)
 
 section \<open>Minimal stuff\<close>
 
-definition points_to :: "(('v, 'a) abs_state \<rightharpoonup> 'r) \<Rightarrow> ('v, 'a) abs_state \<Rightarrow> bool" where
-  "points_to r \<omega> \<longleftrightarrow> (\<exists>hl. r \<omega> = Some hl \<and> has_write_perm_only (get_state \<omega>) hl )"
+(*
+definition points_to where
+  "points_to r = { \<omega> |\<omega> hl. r \<omega> = Some hl \<and> has_write_perm_only (get_abs_state \<omega>) hl}"
 
 definition points_to_value where
-  "points_to_value r e \<omega> \<longleftrightarrow>(\<exists>hl v. r \<omega> = Some hl \<and> e \<omega> = Some v \<and> has_write_perm_only (get_state \<omega>) hl \<and> has_value (get_state \<omega>) hl v)"
-
+  "points_to_value r e = { \<omega> |\<omega> hl v. r \<omega> = Some hl \<and> e \<omega> = Some v \<and> has_write_perm_only (get_abs_state \<omega>) hl \<and> has_value (get_abs_state \<omega>) hl v}"
+*)
+(*
 definition atrue :: "('v, 'a) abs_state assertion" where
   "atrue \<omega> \<longleftrightarrow> True"
-
-definition assertify :: "('v, 'a) abs_state set \<Rightarrow> ('v, 'a) abs_state assertion" where
-  "assertify S \<omega> \<longleftrightarrow> stabilize \<omega> \<in> S"
-
+*)
 
 section \<open>Something else\<close>
 
@@ -277,47 +643,192 @@ abbreviation univ :: "'a \<Rightarrow> ('v, 'a) abs_state set" where
 
 
 
-definition exists_assert :: "('v, 'r) abs_type_context \<Rightarrow> var \<Rightarrow> ('v, 'a) abs_state assertion \<Rightarrow> ('v, 'a) abs_state assertion" where
-  "exists_assert \<Delta> x A \<omega> \<longleftrightarrow> (\<exists>v0 v ty. v0 \<in> ty \<and> get_store \<omega> x = Some v0 \<and> variables \<Delta> x = Some ty \<and> v \<in> ty \<and> A ((Ag ((get_store \<omega>)(x := Some v)), Ag (get_trace \<omega>)), get_state \<omega>))"
+\<comment> \<open>Hongyi defined these 3 functions for his thesis.
+\<^const>\<open>framed_by_exp\<close> doesn't fully characterize the property "assertion \<^term>\<open>A\<close> frames expression \<^term>\<open>e\<close>",
+in the sense that although \<^term>\<open>e (stabilize_state \<omega>)\<close> has value, it may not equal to \<^term>\<open>e \<omega>\<close>.
+In addition to "frame expression" property, it also excludes evaluation error case. For example,
+expression \<^term>\<open>1 / x\<close> is framed by any assertion, but atrue does not \<^const>\<open>framed_by_exp\<close>
+it by definition, as there is evaluation error when \<^prop>\<open>x = 0\<close> and it evaluates to \<^const>\<open>None\<close> then.
+Nevertheless, this additional characterization is also essential in defining LocalAssign rule when
+choosing to do substitution in post-condition: this LocalAssign statement must reduce every state
+satisfying pre-condition. As a result, every state satisfying pre-condition must evaluate the expression
+\<^term>\<open>e\<close> not to \<^const>\<open>None\<close>, which is exactly characterized by \<^const>\<open>framed_by_exp\<close>. Moreover,
+substitute_state should be used only when \<^prop>\<open>e \<omega> \<noteq> None\<close>. In SL rules, this is guaranteed by \<^const>\<open>framed_by_exp\<close>.
+\<close>
+
+(*
+definition assertion_frame_exp :: "('v, 'a) abs_state assertion \<Rightarrow> (('v, 'a) abs_state, 'v) exp \<Rightarrow> bool" where
+  "assertion_frame_exp A e \<longleftrightarrow> (\<forall>\<omega> \<in> A. e \<omega> = e (stabilize \<omega>))"
+*)
+
+definition substitute_var_state where
+  "substitute_var_state x e \<omega> = assign_var_state x (e \<omega>) \<omega>"
+
+definition post_substitute_var_assert :: "var \<Rightarrow> (('v, 'a) abs_state, 'v) exp \<Rightarrow> ('v, 'a) abs_state assertion \<Rightarrow> ('v, 'a) abs_state assertion" where
+  "post_substitute_var_assert x e A = substitute_var_state x e ` A"
+
+(*
+definition set_value_state :: "'r \<Rightarrow> 'v \<Rightarrow> ('v, 'a) abs_state \<Rightarrow> ('v, 'a) abs_state" where
+  "set_value_state l v \<omega> = ((Ag (get_store \<omega>), Ag (get_trace \<omega>)), set_value (get_abs_state \<omega>) l v)"
+*)
+
+(*
+definition substitute_field_state :: "(('v, 'a) abs_state \<rightharpoonup> 'r) \<Rightarrow> (('v, 'a) abs_state, 'v) exp \<Rightarrow> ('v, 'a) abs_state \<Rightarrow> ('v, 'a) abs_state" where
+  "substitute_field_state r e \<omega> = set_abs_state \<omega> (set_value (get_abs_state \<omega>) (the (r \<omega>)) (the (e \<omega>)))"
+
+definition post_substitute_field_assert :: "(('v, 'a) abs_state \<rightharpoonup> 'r) \<Rightarrow> (('v, 'a) abs_state, 'v) exp \<Rightarrow> ('v, 'a) abs_state assertion \<Rightarrow> ('v, 'a) abs_state assertion" where
+  "post_substitute_field_assert r e A = { \<omega>' |\<omega>' \<omega>. \<omega> \<in> A \<and> \<omega>' = substitute_field_state r e \<omega>}"
+*)
+
+
+
+(*
+lemma assertion_frames_exp_eq:
+  assumes "wf_exp e"
+      and "self_framing A"
+      and "framed_by_exp A e"
+    shows "assertion_frame_exp A e"
+  unfolding assertion_frame_exp_def
+proof
+  fix \<omega> assume asm0: "\<omega> \<in> A"
+  then have "stabilize \<omega> \<in> A"
+    using assms(2) self_framing_def by auto
+  then obtain v where "e (stabilize \<omega>) = Some v"
+    by (metis assms(3) framed_by_exp_def option.collapse)
+  then show "e \<omega> = e (stabilize \<omega>)"
+    by (metis (no_types, lifting) assms(1) decompose_stabilize_pure greater_def wf_expE)
+qed
+*)
+
+
 
 section \<open>SL Proof\<close>
 
+(*
 definition depends_on_ag_store_only where
   "depends_on_ag_store_only e \<longleftrightarrow> (\<forall>\<sigma> \<gamma> \<gamma>'. e (\<sigma>, \<gamma>) = e (\<sigma>, \<gamma>'))"
+*)
+(*
+set_abs_state \<omega> (set_value (get_abs_state \<omega>) (the (r \<omega>)) (the (e \<omega>)))"
+*)
+(*
+(* \<exists>l v. b[r \<rightarrow> v] \<inter> r = e[r \<rightarrow> v] 
+r and *r
+TODO TODO TODO
+*)
 
-inductive SL_proof :: "('v, 'r) abs_type_context \<Rightarrow> ('v, 'a) abs_state assertion \<Rightarrow> (('v, 'a) abs_state, 'v, 'r) abs_stmt \<Rightarrow> ('v, 'a) abs_state assertion \<Rightarrow> bool"
+*)
+
+(* What if r depends on e? b can also mention this! *)
+
+(* \<omega>' is the old state! *)
+(*
+definition pure_post_field_assign where
+  "pure_post_field_assign r e b = { \<omega> |\<omega> l v. let \<omega>' = set_abs_state \<omega> (set_value (get_abs_state \<omega>) l v) in
+  (b \<omega>' = Some True \<and> has_write_perm_only (get_abs_state \<omega>) (the (r \<omega>')) \<and> has_value (get_abs_state \<omega>) (the (r \<omega>')) (the (e \<omega>')))}"
+*)
+abbreviation self_framing_and_typed where
+  "self_framing_and_typed \<Delta> A \<equiv> self_framing_typed \<Delta> A \<and> typed_assertion \<Delta> A"
+
+
+definition pure_typed where
+  "pure_typed \<Delta> b = { \<omega> |\<omega>. b \<omega> = Some True \<and> pure \<omega> \<and> typed \<Delta> \<omega> }"
+
+lemma typed_assertion_pure_typed:
+  "typed_assertion \<Delta> (pure_typed \<Delta> b)"
+  using pure_typed_def typed_assertionI
+  by (metis (no_types, lifting) CollectD)
+
+
+inductive SL_proof :: "('v, 'c) abs_type_context \<Rightarrow> ('v, 'a) abs_state assertion \<Rightarrow> (('v, 'a) abs_state, 'v, 's) abs_stmt \<Rightarrow> ('v, 'a) abs_state assertion \<Rightarrow> bool"
    ("_ \<turnstile> [_] _ [_]" [51,0,0] 81)
    where
 
-  RuleSkip: "self_framing A \<Longrightarrow> _ \<turnstile> [A] Skip [A]"
+  RuleSkip: "self_framing_and_typed \<Delta> A \<Longrightarrow> \<Delta> \<turnstile> [A] Skip [A]"
 \<comment>\<open>Because no frame rule, needs A on both sides.\<close>
 
-| RuleInhale: "self_framing A \<Longrightarrow> framed_by A P \<Longrightarrow> _ \<turnstile> [A] Inhale P [A && P]"
+| RuleInhale: "self_framing_and_typed \<Delta> A \<Longrightarrow> framed_by A P \<Longrightarrow> \<Delta> \<turnstile> [A] Inhale P [A \<otimes> P]"
 \<comment>\<open>P framed by A ensures that A && P is self-framing.\<close>
 
-| RuleExhale: "self_framing B \<Longrightarrow> entails B (A && P) \<Longrightarrow> self_framing A \<Longrightarrow> _ \<turnstile> [B] Exhale P [A]"
+| RuleExhale: "self_framing_and_typed \<Delta> B \<Longrightarrow> entails B (A \<otimes> P) \<Longrightarrow> self_framing_and_typed \<Delta> A \<Longrightarrow> \<Delta> \<turnstile> [B] Exhale P [A]"
+
 \<comment>\<open>Exhale can lose information, because we're forced to factorize the set, which is why the entails is needed.
 Example:
 {a1 + p1, a2 + p2} \<longlonglongrightarrow> {a1, a2}
 <A * P> = {a1 + p1, a2 + p2, a1 + p2, a2 + p1} \<longlonglongrightarrow> {a1, a2}\<close>
 
-| RuleAssert: "self_framing A \<Longrightarrow> entails A P \<Longrightarrow> _ \<turnstile> [A] Assert P [A]"
+| RuleAssert: "self_framing_and_typed \<Delta> A \<Longrightarrow> entails A P \<Longrightarrow> \<Delta> \<turnstile> [A] Assert P [A]"
 \<comment>\<open>Assert does not behave like exhale: It forces the *whole* heap to satisfy P.
 Because there is not frame rule, it can be used to express leak checks, or absence of obligations.\<close>
 
-| RuleHavoc: "self_framing A \<Longrightarrow> \<Delta> \<turnstile> [A] Havoc x [exists_assert \<Delta> x A]"
-(*
-| RuleHavoc: "self_framing A \<Longrightarrow> self_framing B \<Longrightarrow> entails A B \<Longrightarrow> free_vars \<Delta> B \<subseteq> free_vars \<Delta> A - {x} \<Longrightarrow> \<Delta> \<turnstile> [A] Havoc x [B]"
-*)
+| RuleAssume: "self_framing_and_typed \<Delta> A \<Longrightarrow> self_framing_on A P \<Longrightarrow> \<Delta> \<turnstile> [A] Assume P [A \<inter> P]"
+
+
+| RuleHavoc: "self_framing_and_typed \<Delta> A \<Longrightarrow> \<Delta> \<turnstile> [A] Havoc x [exists_assert \<Delta> x A]"
+
 \<comment>\<open>Entails needed, because we lose information. The strongest post might be \<exists>x. A, but does not seem more useful.\<close>
 
+\<comment> \<open>
 | RuleFieldAssignHeapIndep:
   "\<lbrakk> self_framing A; framed_by_exp A r; framed_by_exp A e; depends_on_ag_store_only r; depends_on_ag_store_only e \<rbrakk>
   \<Longrightarrow> \<Delta> \<turnstile> [A && points_to r] FieldAssign r e [A && points_to_value r e]"
+Replaced by the new uniform one below in Hongyi's thesis.\<close>
+
+ (* ; assertion_frame_exp (A \<otimes> points_to r) e *)
+(* Precondition should be A \<otimes> points_to_r e' for some e', framed_by A *)
+
+(* Cannot split acc(x.f) * acc(y.f) * x.f = y.f *)
+(* Needs a pure equation b on the side *)
+(* or entails... *)
+
+(*
+| RuleFieldAssignWithEntails: "\<lbrakk> entails B (A \<otimes> points_to r); self_framing A; framed_by_exp (A \<otimes> points_to r) b; framed_by_exp (A \<otimes> points_to r) e \<rbrakk>
+  \<Longrightarrow> _ \<turnstile> [B] FieldAssign r e [post_substitute_field_assert r e (A \<otimes> points_to r)]"
+*)
 
 
+(* Postcondition should be:
+A \<otimes> points_to r \<otimes> (\<exists>v. b[r \<rightarrow> v] \<inter> r = e[r \<rightarrow> v])
+*)
+
+
+(*
+| RuleFieldAssignOld: "\<lbrakk> self_framing (A \<otimes> points_to r); framed_by_exp (A \<otimes> points_to r) e \<rbrakk>
+  \<Longrightarrow> _ \<turnstile> [A \<otimes> points_to r] FieldAssign r e [post_substitute_field_assert r e (A \<otimes> points_to r)]"
+*)
+
+\<comment> \<open>Replaced to the new one above in Hongyi's thesis. The new one simply simulates reduction of this statement,
+  with assumptions ensuring the simulation doesn't cause error.
 | RuleFieldAssign: "\<lbrakk> self_framing (A && points_to_value r e') ; framed_by_exp (A && points_to r) e \<rbrakk>
-  \<Longrightarrow> \<Delta> \<turnstile> [A && points_to_value r e'] FieldAssign r e [A && points_to_value r e]"
+  \<Longrightarrow> \<Delta> \<turnstile> [A && points_to_value r e'] FieldAssign r e [A && points_to_value r e]"\<close>
+
+
+
+\<comment> \<open>
+| RuleLocalAssign: "\<lbrakk> self_framing A; framed_by_exp A e; x \<notin> free_vars \<Delta> A \<rbrakk> \<Longrightarrow>  \<Delta> \<turnstile> [A] LocalAssign x e [ A && var_equal_exp x e ]"
+Change to new one for Hongyi's thesis. The reason not to do substitution in precondition is that it is hard to express framing requirements.
+Intuitively, since \<^term>\<open>e\<close> is not evaluated in post-condition, it is not reasonable to express "post-condition \<^term>\<open>A\<close> frames \<^term>\<open>e\<close>".
+Assuming "A[x \<mapsto> e] frames e" makes the rule even more complicated than the one below.
+Moreover, \<^prop>\<open>framed_by_exp A e\<close> doesn't work here: assume we want to have rule as "\<turnstile> {A[x \<mapsto> e]} x := e {A}",
+then simply requiring \<^prop>\<open>framed_by_exp A e\<close> is wrong: due to the additional characterization of evaluation error case of \<^const>\<open>framed_by_exp\<close>,
+this rule cannot express "\<turnstile> {x \<noteq> 0} x := 0/x {x = 0}" (if \<^term>\<open>A\<close> is \<^prop>\<open>x = 0\<close>,
+then "0/x" always evaluates to \<^const>\<open>None\<close>, and \<^term>\<open>A\<close> can never \<^const>\<open>framed_by_exp\<close> "0/x").
+Explanation of assumptions:
+- To guarantee that \<^const>\<open>assign_var_state\<close> works under \<^prop>\<open>e \<omega> \<noteq> None\<close>, \<^prop>\<open>framed_by_exp A e\<close> is necessary.
+- To get self-framingness of post-condition, \<^prop>\<open>assertion_frame_exp A e\<close> is necessary.
+This rule is sound because: for every state \<^term>\<open>\<omega>\<close> satisfying \<^term>\<open>A\<close>. \<^term>\<open>e \<omega>\<close> evaluates to \<^term>\<open>Some v\<close>, and for the post-state \<^term>\<open>\<omega>'\<close>, the existence of \<^term>\<open>\<omega>\<close> makes it satisfy \<^term>\<open>post_substitute_assert x e A\<close>.
+This rule should be complete (maybe not yet): as long as the LocalAssign statement reduces for pre-condition \<^term>\<open>A\<close>, \<^term>\<open>e\<close> must evaluate to not \<^const>\<open>None\<close> for every state in \<^term>\<open>A\<close>, thus \<^prop>\<open>framed_by_exp A e\<close>. \<^prop>\<open>assertion_frame_exp A e\<close> is a framing requirement, and a correct reduction should satisfy it.
+\<close>
+| RuleLocalAssign: "\<lbrakk> self_framing_and_typed \<Delta> A; framed_by_exp A e \<rbrakk> \<Longrightarrow> \<Delta> \<turnstile> [A] LocalAssign x e [post_substitute_var_assert x e A]"
+
+(*
+  assumes "wf_exp e"
+      and "self_framing A"
+      and "framed_by_exp A e"
+    shows "assertion_frame_exp A e"
+*)
+
+
 \<comment>\<open>Like inhale and the if rule, needs to frame r and e.
 Interestingly, does not work if we only have
 - self_framing A
@@ -342,10 +853,6 @@ x.f := ...
 [e] := ...
 --> "issue" if location of "e" depends on the value of e
 
-
-
-
-
 x.f.f := ...
 --> "issue" if location of "x.f.f" depends on the value of x.f.f
 --> In Viper, location of "x.f.f" depends on the value of x.f
@@ -362,18 +869,12 @@ x = 0 && (\<exists>v. x.f \<mapsto> v /\ v
 acc(x.f) && x.f = x
 [x.f.f := ...]
 
-
-
-Might need an entailment...
-
-Otherwise:
-\<close>
+Might need an entailment...\<close>
 
 | RuleSeq: "\<lbrakk> \<Delta> \<turnstile> [A] C1 [R] ; \<Delta> \<turnstile> [R] C2 [B] \<rbrakk> \<Longrightarrow> \<Delta> \<turnstile> [A] Seq C1 C2 [B]"
-| RuleIf: "\<lbrakk> framed_by_exp A b; \<Delta> \<turnstile> [A \<and>\<and> (pure_assertify b)] C1 [B1] ; \<Delta> \<turnstile> [A \<and>\<and> (pure_assertify (negate b))] C2 [B2] \<rbrakk>
-  \<Longrightarrow> \<Delta> \<turnstile> [A] If b C1 C2 [B1 || B2]"
 
-
+| RuleIf: "\<lbrakk> self_framing_and_typed \<Delta> A; framed_by_exp A b; \<Delta> \<turnstile> [A \<otimes> pure_typed \<Delta> b] C1 [B1] ; \<Delta> \<turnstile> [A \<otimes> pure_typed \<Delta> (negate b)] C2 [B2] \<rbrakk>
+  \<Longrightarrow> \<Delta> \<turnstile> [A] If b C1 C2 [B1 \<union> B2]"
 
 (*
 | RuleFrame: "self_framing F \<Longrightarrow> \<Delta> \<turnstile> [A] C [B] \<Longrightarrow> free_var F \<inter> modif C = {} \<Longrightarrow> \<Delta> \<turnstile> [astar A F] C [astar B F]"
@@ -382,20 +883,36 @@ Otherwise:
 | RuleEquiv: "\<lbrakk> equiv A' A ; self_framing A' ; \<Delta> \<turnstile> [A] C [B]; equiv B B'; self_framing B' \<rbrakk> \<Longrightarrow> \<Delta> \<turnstile> [A'] C [B']"
 *)
 
-definition wf_state where
-  "wf_state \<Delta> \<omega> \<longleftrightarrow> (stable \<omega> \<and> typed_store \<Delta> (get_store \<omega>))"
+(*
+| RuleFieldAssign: "\<lbrakk> self_framing A; framed_by_exp A r; framed_by_exp (A \<otimes> points_to r) b; wf_exp b;
+  framed_by_exp (A \<otimes> points_to r \<otimes> pure_Stabilize b) e \<rbrakk>
+  \<Longrightarrow> _ \<turnstile> [A \<otimes> points_to r \<otimes> pure_Stabilize b] FieldAssign r e [A \<otimes> pure_post_field_assign r e b]"
+*)
+| RuleCustom: "\<lbrakk> self_framing_and_typed \<Delta> A; self_framing_and_typed \<Delta> B; SL_Custom \<Delta> A C B \<rbrakk> \<Longrightarrow> \<Delta> \<turnstile> [A] Custom C [B]"
 
-definition wf_set where
-  "wf_set \<Delta> S \<longleftrightarrow> (\<forall>x \<in> S. wf_state \<Delta> x)"
+inductive_cases SL_proof_Skip_elim[elim!]: "\<Delta> \<turnstile> [A] Skip [B]"
+inductive_cases SL_proof_Inhale_elim[elim!]: "\<Delta> \<turnstile> [A] Inhale P [B]"
+inductive_cases SL_proof_Exhale_elim[elim!]: "\<Delta> \<turnstile> [A] Exhale P [B]"
+inductive_cases SL_proof_Assert_elim[elim!]: "\<Delta> \<turnstile> [A] Assert P [B]"
+inductive_cases SL_proof_Havoc_elim[elim!]: "\<Delta> \<turnstile> [A] Havoc x [B]"
+inductive_cases SL_proof_Seq_elim[elim!]: "\<Delta> \<turnstile> [A] Seq C1 C2 [B]"
+inductive_cases SL_proof_If_elim[elim!]: "\<Delta> \<turnstile> [A] If b C1 C2 [B]"
+inductive_cases SL_proof_Custom_elim[elim!]: "\<Delta> \<turnstile> [A] Custom C [B]"
+
+(*
+inductive_cases SL_proof_FieldAssign_elim[elim!]: "\<Delta> \<turnstile> [A] FieldAssign r e [B]"
+*)
 
 
-definition verifies :: "('v, 'r) abs_type_context \<Rightarrow> (('v, 'a) abs_state, 'v, 'r) abs_stmt \<Rightarrow> ('v, 'a) abs_state \<Rightarrow> bool" where
-  "verifies \<Delta> s \<omega> \<longleftrightarrow> (\<exists>S. red_stmt \<Delta> s \<omega> S)"
+
+
+
+definition verifies :: "('v, 'c) abs_type_context \<Rightarrow> (('v, 'a) abs_state, 'v, 's) abs_stmt \<Rightarrow> ('v, 'a) abs_state \<Rightarrow> bool" where
+  "verifies \<Delta> C \<omega> \<longleftrightarrow> (\<exists>S. red_stmt \<Delta> C \<omega> S)"
 
 (* \<omega> is pure? *)
-definition verifies_rel where
-  "verifies_rel \<Delta> A C \<longleftrightarrow> (\<forall>\<omega> \<in> \<langle>A\<rangle>. stable \<omega> \<longrightarrow> (\<exists>S. red_stmt \<Delta> C \<omega> S))"
-
+definition verifies_set where
+  "verifies_set \<Delta> A C \<longleftrightarrow> (\<forall>\<omega> \<in> A. stable \<omega> \<and> typed \<Delta> \<omega> \<longrightarrow> verifies \<Delta> C \<omega>)"
 
 
 end
