vipersemcommon/SepAlgebra.thy
@@ -105,6 +105,29 @@ next
   then show ?A
     using greater_def by auto
 qed
+lemma comp_prod:
+  "a ## b \<longleftrightarrow> (fst a ## fst b \<and> snd a ## snd b)" (is "?A \<longleftrightarrow> ?B")
+proof
+  assume ?A
+  then obtain x where "Some x = a \<oplus> b"
+    by (metis defined_def not_Some_eq)
+  then have "Some (fst x) = fst a \<oplus> fst b \<and> Some (snd x) = snd a \<oplus> snd b"
+    by (metis SepAlgebra.plus_prodE)
+  then show ?B
+    by (metis defined_def option.discI)
+next
+  assume ?B
+  then obtain r1 r2 where "Some r1 = fst a \<oplus> fst b \<and> Some r2 = snd a \<oplus> snd b"
+    by (metis defined_def option.exhaust_sel)
+  then show ?A
+    using defined_def SepAlgebra.plus_prodIAlt by fastforce
+qed    
+
+lemma compatible_prodI:
+  assumes "fst a ## fst b"
+      and "snd a ## snd b"
+    shows "a ## b"
+  using assms(1) assms(2) comp_prod by blast
 
 end
 
@@ -112,11 +135,19 @@ subsection \<open>Function\<close>
 
 datatype 'v agreement = Ag (the_ag: 'v)
 
+
 instantiation "agreement" :: (type) pcm
 begin
 
 definition plus_agreement :: "'a agreement \<Rightarrow> 'a agreement \<Rightarrow> 'a agreement option" where
   "plus_agreement a b = (if a = b then Some a else None)"
+
+lemma plus_AgI:
+  fixes \<omega> :: "'v agreement"
+  assumes "\<omega> = a"
+      and "\<omega> = b"
+    shows "Some \<omega> = a \<oplus> b"
+  by (metis SepAlgebra.plus_agreement_def assms(1) assms(2))
 
 instance proof
   fix a b c ab bc :: "'a agreement"
@@ -129,6 +160,11 @@ instance proof
   show "a \<oplus> b = Some c \<Longrightarrow> Some c = c \<oplus> c \<Longrightarrow> Some a = a \<oplus> a "
     by (metis plus_agreement_def)
 qed
+
+lemma greater_Ag:
+  fixes a b :: "'a agreement"
+  shows "a \<succeq> b \<longleftrightarrow> a = b"
+  by (simp add: SepAlgebra.plus_agreement_def greater_def)
 
 
 end
